syntax to define programs

Pop/States.lean
@@ -4,15 +4,23 @@ open Util
 namespace Pop
 
 def RequestId := Nat deriving ToString, BEq
-def Value := Nat deriving ToString, BEq
+def Value := Option Nat deriving ToString, BEq
 def Address := Nat deriving ToString, BEq
 def ThreadId := Nat deriving BEq, Ord, LT, LE, ToString
 
 def RequestId.toNat : RequestId → Nat := λ x => x
+def ThreadId.toNat : RequestId → Nat := λ x => x
+def RequestId.ofNat : Nat → RequestId := λ x => x
+def ThreadId.ofNat : Nat → RequestId := λ x => x
+def Address.ofNat : Nat → Address := λ x => x
+
+instance : OfNat ThreadId n where  ofNat := ThreadId.ofNat n
+instance : OfNat RequestId n where  ofNat := RequestId.ofNat n
+instance : OfNat Address n where ofNat := Address.ofNat n
 
 structure ReadRequest where
  addr : Address
- reads_from : RequestId
+ reads_from : Option RequestId
  val : Value
 
 structure WriteRequest where
@@ -24,10 +32,19 @@ inductive BasicRequest
  | write : WriteRequest → BasicRequest
  | barrier : BasicRequest
 
--- TODO: write properly
+def mkRead (addr : Address) : BasicRequest :=
+  let rr : ReadRequest := { addr := addr, reads_from := none, val := none}
+  BasicRequest.read rr
+
+def mkWrite (addr : Address) : BasicRequest :=
+  let wr : WriteRequest := { addr := addr, val := none}
+  BasicRequest.write wr
+
+def mkBarrier : BasicRequest := BasicRequest.barrier
+
 def BasicRequest.toString
-  | BasicRequest.read  _ => "read"
-  | BasicRequest.write _ => "write"
+  | BasicRequest.read  rr => s!"read ({rr.addr})"
+  | BasicRequest.write  wr => s!"write ({wr.addr})"
   | BasicRequest.barrier => "barrier"
 instance : ToString BasicRequest where toString := BasicRequest.toString
 
@@ -38,12 +55,17 @@ structure Request where
   basic_type : BasicRequest
   -- type : α
 
+def Request.toString : Request → String
+  | req => s!" Request {req.id} {req.basic_type} : [propagated to {req.propagated_to}, origin thread : {req.thread}]"
+instance : ToString Request where toString := Request.toString
+
 def BasicRequest.isRead    (r : BasicRequest) : Bool := match r with | read  _ => true | _ => false
 def BasicRequest.isWrite   (r : BasicRequest) : Bool := match r with | write _ => true | _ => false
 def BasicRequest.isBarrier (r : BasicRequest) : Bool := match r with | barrier => true | _ => false
 def Request.isRead    (r : Request) : Bool := r.basic_type.isRead
 def Request.isWrite   (r : Request) : Bool := r.basic_type.isWrite
 def Request.isBarrier (r : Request) : Bool := r.basic_type.isBarrier
+def Request.isMem     (r : Request) : Bool := !r.basic_type.isBarrier
 
 def BasicRequest.address? (r : BasicRequest) : Option Address := match r with
   | read  req => some req.addr
@@ -92,6 +114,8 @@ def System.threads : System → List ThreadId
 
 def OrderConstraints {V : ValidScopes} :=  (@Scope V) → RequestId → RequestId → Bool
 
+def OrderConstraints.empty {V : ValidScopes}  : @OrderConstraints V := λ _ _ _ => true
+
 def OrderConstraints.predecessors {V : ValidScopes} (S : @Scope V) (req : RequestId)
     (reqs : List RequestId) (constraints : @OrderConstraints V)  : List RequestId :=
     reqs.filter (λ x => constraints S x req)
@@ -128,12 +152,15 @@ structure RequestArray where
   val : Array (Option Request)
   coherent : valConsistent val = true
 
-def filterNones {α : Type} : List (Option α) → List α
-  | none::rest => filterNones rest
-  | (some val):: rest => val::(filterNones rest)
-  | [] => []
+theorem emptyArrayCoherent : valConsistent (Array.mk []) := by simp
+def RequestArray.empty : RequestArray :=
+  { val := Array.mk [], coherent := emptyArrayCoherent }
 
-private def reqIds : RequestArray → List RequestId
+def RequestArray.toString : RequestArray → String
+  | arr => String.intercalate "\n" $ List.map Request.toString $ filterNones arr.val.toList
+instance : ToString RequestArray where toString := RequestArray.toString
+
+def reqIds : RequestArray → List RequestId
  | arr =>
    let opIds :=  Array.toList $ arr.val.map (Option.map Request.id)
    filterNones opIds
@@ -178,116 +205,32 @@ structure SystemState where
   removedCoherent : ∀ id : RequestId, id ∈ removed → id ∈ reqIds requests
   satisfiedCoherent : ∀ id₁ id₂ : RequestId, (id₁,id₂) ∈ satisfied → id₁ ∈ seen ∧ id₂ ∈ seen
 
-inductive Transition
-  | acceptRequest : BasicRequest → ThreadId → Transition
-  | propagateToThread : RequestId → ThreadId → Transition
-  | satisfyRead : RequestId → RequestId → Transition
+def SystemState.toString : SystemState → String
+  | state => s!"requests:\n{state.requests.toString}\n"  ++
+  s!"seen: {state.seen.toString}\n" ++
+  s!"removed: {state.removed.toString}\n" ++
+  s!"satisfied: {state.satisfied.toString}\n"
+
+theorem emptyCoherent (requests : RequestArray) :
+  ∀ id : RequestId, id ∈ [] → id ∈ reqIds requests := by
+  intros id h
+  contradiction
+
+theorem empty2Coherent (seen : List RequestId) :
+  ∀ id₁ id₂ : RequestId, (id₁,id₂) ∈ [] → id₁ ∈ seen ∧ id₂ ∈ seen := by
+  intros
+  contradiction
+
+def SystemState.init (S : System) : SystemState :=
+  { requests := RequestArray.empty, seen := [], removed := [],
+    system := S, satisfied := [], orderConstraints := OrderConstraints.empty,
+    seenCoherent := emptyCoherent RequestArray.empty,
+    removedCoherent := emptyCoherent RequestArray.empty,
+    satisfiedCoherent := empty2Coherent []
+  }
 
 def SystemState.idsToReqs : SystemState → List RequestId → List Request
   | state, ids => filterNones $ ids.map (λ id => state.requests.val[id])
-
-def SystemState.canAcceptRequest : SystemState → BasicRequest → ThreadId → Bool
- | _, _, _ => true
-
-def SystemState.acceptRequest : SystemState → BasicRequest → ThreadId → SystemState
-  | state, reqType, tId =>
-  let req : Request := { propagated_to := [tId], thread := tId, basic_type := reqType, id := state.requests.val.size}
-  let requests' := state.requests.insert req
-  { requests := requests', system := state.system, seen := state.seen,
-    orderConstraints := state.orderConstraints,
-    removed := state.removed, satisfied := state.satisfied,
-    seenCoherent := sorry
-    removedCoherent := sorry
-    satisfiedCoherent := state.satisfiedCoherent
-  }
-
-def SystemState.updateOrderConstraints (state : SystemState) : @Scope state.system.scopes → RequestId → ThreadId → @OrderConstraints state.system.scopes
-  | scope, reqId, thId =>
-  match state.requests.val[reqId] with
-    | none => state.orderConstraints
-    | some req =>
-      let pred := state.idsToReqs $ state.orderConstraints.predecessors scope reqId (reqIds state.requests)
-      let predReorder := pred.filter λ r => state.system.reorder_condition r req
-      let predThread := predReorder.filter λ r => r.propagatedTo thId
-      let newConstraints := [reqId].zip $ predThread.map Request.id
-      state.orderConstraints.append scope newConstraints
-
-def Request.isPropagated? : Request → ThreadId → Bool
-  | req, thId => req.propagated_to.elem thId
-
-def SystemState.canPropagate : SystemState → RequestId → ThreadId → Bool
-  | state, reqId, thId =>
-  match state.requests.val[reqId] with
-  | none => false
-  | some req =>
-    let unpropagated := req.isPropagated? thId
-    let scope := state.system.scopes.jointScope thId req.thread
-    let pred := state.orderConstraints.predecessors scope reqId (reqIds state.requests)
-    let reqOps := state.requests.val.filter (λ req => match req with | none => false | some r => pred.elem r.id)
-    let reqs := filterNones reqOps.toList
-    let predPropagated := reqs.map (λ r => r.fullyPropagated state.system.scopes.systemScope)
-    unpropagated || predPropagated.foldl (. && .) true
-
-def Request.propagate : Request → ThreadId → Request
-  | req, thId => { req with propagated_to := thId :: req.propagated_to}
-
-
-def SystemState.propagate : SystemState → RequestId → ThreadId → SystemState
-  | state, reqId, thId =>
-  let reqOpt := state.requests.val[reqId]
-  match reqOpt with
-  | none => state
-  | some req =>
-    let requests' := state.requests.insert (req.propagate thId)
-    let scope := state.system.scopes.jointScope thId req.thread
-    let orderConstraints' := state.updateOrderConstraints scope reqId thId
-    { requests := requests', orderConstraints := orderConstraints',
-      seen := state.seen, removed := state.removed, satisfied := state.satisfied,
-      seenCoherent := sorry, removedCoherent := sorry,
-      satisfiedCoherent := state.satisfiedCoherent
-    }
-
-def SystemState.canSatisfyRead : SystemState → RequestId → RequestId → Bool
-  | state, readId, writeId =>
-  if (state.satisfied.map λ x => x.1).elem readId then false else
-  match state.requests.val[readId], state.requests.val[writeId] with
-    | some read, some write =>
-      let scope := state.system.scopes.jointScope read.thread write.thread
-      let betweenIds := state.orderConstraints.between scope read.id write.id (reqIds state.requests)
-      let between := state.idsToReqs betweenIds
-      let writesToAddrBetween := between.filter (λ r => r.isWrite && r.address? == write.address?)
-      writesToAddrBetween.length == 0
-    | _, _ => false
-
-def SystemState.satisfy : SystemState → RequestId → RequestId → SystemState
- | state, readId, writeId =>
- let satisfied' := (readId,writeId)::state.satisfied
- let removed' :=  readId::state.removed
- let requests' := state.requests.remove readId
- let orderConstraints' := state.orderConstraints.purge readId
- { requests := requests', orderConstraints := orderConstraints',
-   removed := removed', satisfied := satisfied',
-   seen := state.seen, seenCoherent := sorry, removedCoherent := sorry,
-   satisfiedCoherent := sorry
- }
-
-open Transition in
-def SystemState.applyTransition : SystemState → Transition → Except String SystemState
-  | state, (.acceptRequest req tId) =>
-    if (state.canAcceptRequest req tId)
-    then Except.ok $ state.acceptRequest req tId
-    else throw s!"Invalid transition. Can't accept request {req} to Thread {tId}"
-  | state, .propagateToThread reqId tId =>
-    if (state.canPropagate reqId tId)
-    then Except.ok $ state.propagate reqId tId
-    else throw s!"Invalid transition. Can't propagate Request {reqId} to Thread {tId}"
-  | state, satisfyRead readId writeId =>
-    if (state.canSatisfyRead readId writeId)
-    then Except.ok $ state.satisfy readId writeId
-    else throw s!"Invalid transition. Can't satisfy Request {readId} with {writeId}"
-
-def SystemState.applyTrace : SystemState → List Transition → Except String SystemState
-  | state, transitions => transitions.foldlM SystemState.applyTransition state
 
 -- private def maxThread : ThreadId → List ThreadId → ThreadId
 --   | curmax, n::rest => if curmax < n then maxThread n rest else maxThread curmax rest
