Pop/Program.lean
@@ -1,0 +1,54 @@
+import Pop.States
+import Lean
+import Pop.Pop
+import Pop.Util
+import Std.Data
+open Std.HashMap
+open Util Pop
+
+def mkRequest : String × Address → ThreadId → Option Transition
+  | ("R", addr), thId  => some $ Pop.Transition.acceptRequest (Pop.mkRead addr) thId
+  | ("W", addr), thId  => some $ Pop.Transition.acceptRequest (Pop.mkRead addr) thId
+  | ("Fence", _), thId => some $ Pop.Transition.acceptRequest (Pop.mkBarrier) thId
+  | _, _ => none
+
+def createAcceptList : List (List (String × String)) → List Transition
+  | list =>
+  let variablesRaw := list.map λ thread => thread.map (λ r => if r.2.length == 0 then none else some r.2)
+  let variables := removeDuplicates $ filterNones $ List.join variablesRaw
+  let variableNums := variables.zip (List.range variables.length)
+  let variableMap := Std.mkHashMap (capacity := variableNums.length) |> variableNums.foldl λ acc (k, v) => acc.insert k v
+  let replaceVar := λ (req,var) => (req, 1 + (Option.get! $ variableMap.find? var))
+  let replacedVariables : List (List (String × Nat)) := list.map λ thread => thread.map replaceVar
+  let fullThreads := replacedVariables.zip (List.range replacedVariables.length)
+  let mkThread := λ (reqs, thId) => filterNones $ reqs.map (λ r => mkRequest r thId)
+  List.join $ fullThreads.map mkThread
+
+declare_syntax_cat request
+declare_syntax_cat request_seq
+declare_syntax_cat request_set
+syntax "R" ident : request
+syntax "W" ident : request
+syntax "Fence"   : request
+syntax request ";" request_seq : request_seq
+syntax request : request_seq
+syntax request_seq "||" request_set : request_set
+syntax request_seq : request_set
+syntax "<|" request_set "|>" : term
+
+-- syntax sepBy(request_seq,  "||") : request_set
+
+macro_rules
+ | `(request| R $x:ident) => `(("R", $(Lean.quote x.getId.toString)))
+ | `(request| W $x:ident) => `(("W", $(Lean.quote x.getId.toString)))
+ | `(request| Fence     ) => `(("Fence", ""))
+
+macro_rules
+  | `(request_seq| $r:request ) => `([$r])
+  | `(request_seq| $r:request ; $rs:request_seq) => `($r :: $rs)
+
+macro_rules
+  | `(request_set| $r:request_seq ) => `([$r])
+  | `(request_set| $r:request_seq || $rs:request_set) => `($r :: $rs)
+macro_rules
+  | `(<| $r |>) => `( createAcceptList $r)
